Wavelet/Semantics/PCM.lean
@@ -6,12 +6,10 @@ class PCM (C : Type u) where
   add : C → C → C
   zero : C
   valid : C → Prop
-  eq : C → C → Prop
 
 namespace PCM
 
 infixl:60 " ⊔ " => add
-infix:40 " ≡ " => eq
 prefix:40 "✓ " => valid
 
 def disjoint [PCM C] (a b : C) : Prop := ✓ a ⊔ b
@@ -26,46 +24,27 @@ infix:50 " ⊥ " => disjoint
 infix:50 " ⟹ " => framePreserving
 
 instance [PCM C] : LE C where
-  le a b := ∃ c, b ≡ a ⊔ c
+  le a b := ∃ c, b = a ⊔ c
 
 noncomputable def sub [PCM C] (a b : C) (hle : b ≤ a) : C :=
   hle.choose
 
 class Lawful (R : Type u) [inst : PCM R] where
-  add_comm : ∀ {a b : R}, a ⊔ b ≡ b ⊔ a
-  add_assoc : ∀ {a b c : R}, (a ⊔ b) ⊔ c ≡ a ⊔ (b ⊔ c)
-  add_ident : ∀ {a : R}, a ⊔ inst.zero ≡ a
+  add_comm : ∀ {a b : R}, a ⊔ b = b ⊔ a
+  add_assoc : ∀ {a b c : R}, (a ⊔ b) ⊔ c = a ⊔ (b ⊔ c)
+  add_ident : ∀ {a : R}, a ⊔ inst.zero = a
   valid_add : ∀ {a b : R}, ✓ a ⊔ b → ✓ a
   valid_zero : ✓ inst.zero
-  eq_refl : ∀ {a : R}, a ≡ a
-  eq_symm : ∀ {a b : R}, a ≡ b → b ≡ a
-  eq_trans : ∀ {a b c : R}, a ≡ b → b ≡ c → a ≡ c
-  eq_congr_valid : ∀ {a b : R}, a ≡ b → ✓ a → ✓ b
-  eq_congr_add :
-    ∀ {a₁ a₂ b₁ b₂ : R},
-      a₁ ≡ a₂ →
-      b₁ ≡ b₂ →
-      a₁ ⊔ b₁ ≡ a₂ ⊔ b₂
 
-theorem eq_congr_disj
-  [PCM C] [Lawful C]
-  {a₁ a₂ b₁ b₂ : C}
-  (ha : a₁ ≡ a₂)
-  (hb : b₁ ≡ b₂)
-  (hdisj : a₁ ⊥ b₁) :
-    a₂ ⊥ b₂
-  := by
-  simp [disjoint]
-  apply Lawful.eq_congr_valid
-  apply Lawful.eq_congr_add ha hb
-  exact hdisj
+class Cancellative (R : Type u) [PCM R] where
+  cancel_left : ∀ {a b c : R}, a ⊔ b = a ⊔ c → b = c
+  cancel_right : ∀ {a b c : R}, b ⊔ a = c ⊔ a → b = c
 
 /-- PCM homomorphism. -/
 class Hom [instR : PCM R] [instS : PCM S] (h : R → S) where
   hom_zero : h PCM.zero = PCM.zero
-  hom_add : ∀ {a b : R}, h (a ⊔ b) ≡ h a ⊔ h b
+  hom_add : ∀ {a b : R}, h (a ⊔ b) = h a ⊔ h b
   hom_valid : ∀ {a : R}, ✓ a → ✓ h a
-  hom_eq : ∀ {a b : R}, a ≡ b → h a ≡ h b
 
 /-- A trivial PCM with only one element. -/
 inductive Triv where | zero
@@ -74,7 +53,6 @@ instance : PCM Triv where
   add _ _ := Triv.zero
   zero := Triv.zero
   valid _ := True
-  eq _ _ := True
 
 instance : Lawful Triv := by
   constructor
